*use calc functions instead of assert

SquareAndMultiply.dfy
@@ -1,4 +1,4 @@
-function pow(x: int, n: int): int
+opaque function pow(x: int, n: int): int
     requires n >= 0
 {
     if n == 0 then 
@@ -13,7 +13,6 @@ function isEven(a: int): bool
     a % 2 == 0
 }
 
-
 type EvenInt = x: nat | isEven(x) witness 2
 type OddInt = x: nat | !isEven(x) witness 3
 
@@ -23,26 +22,44 @@ ensures r == pow(x, n)
 {
     r := x;
     var tmp := n - 1;
+    calc
+    { 
+        pow(x, n - tmp);        
+        pow(x, n - n + 1);
+        { reveal pow(); }
+        r;
+    }    
     while(tmp > 0)
         invariant r == pow(x, n - tmp)
     {
+        reveal pow();    
         r := r * x;
         tmp := tmp - 1;
     }
 }
 
 lemma AssociativityLaw(x: int, n: int, m: int)
-  requires n > 0
+  requires n >= 0
   requires m >= 0
   ensures pow(x, n + m) == pow(x, n) * pow(x, m)
 {	
     if (m == 0)
     {
-        assert(pow(x, n + 0) == pow(x,n));
+        assert(pow(x, n + 0) == pow(x,n) * pow(x, 0)) by {reveal pow();}
     }
     else
     {
-        AssociativityLaw(x, n, m - 1);
+        calc 
+        {
+            pow(x, n + m);
+            pow(x, n + m - 1 + 1);            
+            { reveal pow(); }
+            pow(x, n + m - 1) * x;  
+            { AssociativityLaw(x, n, m - 1);}
+            pow(x, n) * pow(x, m - 1) * x;   
+            { reveal pow(); }
+            pow(x, n) * pow(x, m);                   
+        }
     }
 }
 
@@ -53,13 +70,29 @@ lemma AssociativityLaw2(x: int, n: int, m: int)
 {
     if (m == 0)
     {
-        assert(pow(x, 0) == 1);
+        calc {
+        pow(x, n * m);
+        { reveal pow(); }
+        1;
+        { reveal pow(); }
+        pow(pow(x, n), 0);
+        }
     }
     else
     {
-        assert(pow(x, n * m) == pow(x, n * (m-1) + n));		
-        AssociativityLaw(x, n, (m-1) * n); // exp(x, m*n) = exp(x, n * (m-1)) * exp(x, n)		
-        AssociativityLaw2(x, n, m - 1);	 // exp(x, n * (m-1)) = exp(exp(x, n), m - 1) 
+        calc 
+        {
+            pow(x, n * m);
+            pow(x, n * (m-1) + n);
+                { AssociativityLaw(x, n, (m-1) * n);} 
+            pow(x, n * (m-1)) * pow(x, n);
+                { AssociativityLaw2(x, n, m - 1);} 
+            pow(pow(x, n), m -1) * pow(x, n);  
+            { reveal pow(); }
+            pow(pow(x, n), m - 1) * pow(pow(x, n), 1);        
+                { AssociativityLaw(pow(x, n), m - 1, 1);} 
+            pow(pow(x, n), m);                
+        }
     }
 }
 
@@ -69,33 +102,37 @@ ensures r == pow(x2, n2)
 {
     var x := x2;
     var n := n2;
-    var y := 1;		
-    assert(y * pow(x, n) == pow(x2, n2));
+    var y := 1; 		
     while (n > 1)
         decreases n
         invariant n > 0
         invariant y * pow(x, n) == pow(x2, n2) 	
-    {			
+    {			    
       if (!isEven(n))
       {
-        AssociativityLaw2(x, 2, (n-1)/2);  // exp(x,n-1) == exp(exp(x, 2), (n-1)/2)     
-        y, x, n := x * y, pow(x, 2), (n-1)/2;	
-        // y * exp(x , n) == y' * exp(x', (n - 1)/2)    
-        // y' = x * y
-        // x' = x * x
-        // zz  	exp(x , n) = x * exp(exp(x, 2), (n-1)/2)
+        calc
+        {
+            y * pow(x, n); 
+           { reveal pow(); }                    
+            pow(x, n - 1)*x; 
+                { AssociativityLaw2(x, 2, (n-1)/2); }             
+            pow(pow(x, 2), (n - 1)/2) * x;   
+        }       
+        y, x, n := x * y, pow(x, 2), (n-1) / 2;	
       }
       else
-      {    
-        AssociativityLaw2(x, 2, n / 2); // exp(x, n) == exp(exp(x, 2), n/2)		
+      { 
+        //reveal pow();             
+        AssociativityLaw2(x, 2, n / 2);	
         y, x, n := y, pow(x, 2), n / 2; 
-        // y * exp(x , n) -> y' * exp(x', n/2)           
-        // y' = y
-        // x' = x * x  
-        // zz  	exp(x , n) = exp(x*x, n/2)
       }	   
+    }   
+    calc
+    {
+        y * pow(x, n) == pow(x2, n2); 	 
+            { reveal pow(); }     
+        y * x == pow(x2, n2);        
     }
-    assert(n == 1);
     r:= x * y; 	
 }
 
